new Tactic

src/evidence.lean
@@ -1,20 +1,21 @@
-import justification fcs common_meta property_catalogue.LTL 
+import justification pump1 common_meta property_catalogue.LTL 
  open S A
 
- @[reducible] def fcs_input_1 : property.input (path fcs) := {property.input .
- Clm := {Claim . X := {x : path fcs | true}, P := λ (π : path fcs), π⊨absent.globally ↑Damaged},
- Props := [λ (π : path fcs), π⊨not_init ↑Damaged, λ (π : path fcs), π⊨holds_over_transition ↑Damaged]}
+ @[reducible] def pump1_input_1 : property.input (path pump1) := {property.input .
+ Clm := {Claim .
+         X := {x : path pump1 | true},
+         P := λ (p : path pump1), p⊨absent.between ↑BolusRequest ↑Cond_6_3_ ↑Infusion_NormalOperation},
+ Props := [λ (p : path pump1), p⊨responds.globally ↑Cond_6_3_ ↑Alrm_EmptyReservoir, λ (p : path pump1),
+              p⊨absent.between ↑BolusRequest ↑Cond_6_3_ ↑Alrm_EmptyReservoir, λ (p : path pump1),
+              p⊨absent.between ↑BolusRequest ↑Alrm_EmptyReservoir ↑Infusion_NormalOperation]}
 
- @[reducible] def fcs_strat_1 : Strategy (path fcs) := property.strategy fcs_input_1
+ @[reducible] def pump1_strat_1 : Strategy (path pump1) := property.strategy pump1_input_1
 
 
-theorem fcs_prf_1 : deductive (path fcs) fcs_strat_1 := 
+theorem pump1_prf_1 : deductive (path pump1) pump1_strat_1 := 
 begin 
-by_induction, 
- base_case P1,
+
 end
 
 
---holds_over_transition ↑Damaged
-
---HINT transitions_safe ↑Damaged
+--responds.globally ↑Cond_6_3_ ↑Alrm_EmptyReservoir
