src/main.lean
@@ -1,22 +1,16 @@
 import justification common_meta property_catalogue.LTL
-import fcs 
+import pump1 
 open interactive S A
-
-
-def foobar : property.input (path fcs) := {}
-
-
-
 
 variable {α : Type}
 
 set_option pp.structure_instances_qualifier true 
 
-def local_input_name : string := "fcs_input_1"
-def local_strat_name : string := "fcs_strat_1"
-def local_prf_name : string := "fcs_prf_1"
+def local_input_name : string := "pump1_input_1"
+def local_strat_name : string := "pump1_strat_1"
+def local_prf_name : string := "pump1_prf_1"
 
-def preamble : string := "import justification fcs common_meta property_catalogue.LTL \n open S A"
+def preamble : string := "import justification pump1 common_meta property_catalogue.LTL \n open S A"
 
 meta def proof_template (p₁ p₂ : string) : string := 
 "\n\n
@@ -25,10 +19,10 @@ theorem " ++ local_prf_name ++ " : " ++ p₁ ++ " := \nbegin \n" ++ p₂ ++ "\ne
 meta def evidence_file_template (ps : PROOF_STATE α) : string := 
 preamble 
 ++ "\n\n @[reducible] def " ++ local_input_name 
-++ " : property.input (path fcs) := "++ ps.input_string
+++ " : property.input (path pump1) := "++ ps.input_string
 ++ "\n\n @[reducible] def "++ local_strat_name 
-++ " : Strategy (path fcs) := property.strategy " ++ local_input_name  
-++ proof_template ("deductive (path fcs) " ++ local_strat_name) (tscript_string ps.tscript)
+++ " : Strategy (path pump1) := property.strategy " ++ local_input_name  
+++ proof_template ("deductive (path pump1) " ++ local_strat_name) (tscript_string ps.tscript)
 ++ ps.unused ++ hints_string ps.hints 
 
 meta def output (s : string) : io unit := do 
@@ -36,7 +30,7 @@ meta def output (s : string) : io unit := do
   io.fs.write of s.to_char_buffer
 
 meta def driver (input : pexpr) : tactic unit := 
-let α := path fcs in 
+let α := path pump1 in 
 let ps : PROOF_STATE α := {} in 
 do 
   STRAT ← tactic.to_expr input,
@@ -51,13 +45,13 @@ do
               strat_expr := STRAT , 
               PROPS := PROPS,
               -- TODO : Clean this
-              init_goal := `(deductive (path fcs) (property.strategy %%STRAT)), 
+              init_goal := `(deductive (path pump1) (property.strategy %%STRAT)), 
               ..ps},
               -- And this
   let ps := get_originals ps,
-  let goal_str := "deductive (path fcs) " ++ local_strat_name,
+  let goal_str := "deductive (path pump1) " ++ local_strat_name,
   set_goal ps.init_goal, 
-  ps ← solve_inductive (ps),
+  ps ← Switch (ps),
   str ← get_unused ps,
     match ps.solved with 
     | tt := tactic.trace "True"
@@ -73,6 +67,84 @@ meta def main
 (meta_info : decl_meta_info)
 (_ : parse (lean.parser.tk "main")) : lean.parser unit :=
 do 
-   F ← read "src/input/Inductive_Example.txt" types.texpr,
+   F ← read "src/input/pumpExample1.txt" types.texpr,
    lean.parser.of_tactic $ driver F
 . 
+
+main
+
+
+-- OLD version, will integrate 
+-- def foobar : property.input (path fcs) := {}
+
+
+
+
+-- variable {α : Type}
+
+-- set_option pp.structure_instances_qualifier true 
+
+-- def local_input_name : string := "fcs_input_1"
+-- def local_strat_name : string := "fcs_strat_1"
+-- def local_prf_name : string := "fcs_prf_1"
+
+-- def preamble : string := "import justification fcs common_meta property_catalogue.LTL \n open S A"
+
+-- meta def proof_template (p₁ p₂ : string) : string := 
+-- "\n\n
+-- theorem " ++ local_prf_name ++ " : " ++ p₁ ++ " := \nbegin \n" ++ p₂ ++ "\nend" ++ "\n\n\n" 
+
+-- meta def evidence_file_template (ps : PROOF_STATE α) : string := 
+-- preamble 
+-- ++ "\n\n @[reducible] def " ++ local_input_name 
+-- ++ " : property.input (path fcs) := "++ ps.input_string
+-- ++ "\n\n @[reducible] def "++ local_strat_name 
+-- ++ " : Strategy (path fcs) := property.strategy " ++ local_input_name  
+-- ++ proof_template ("deductive (path fcs) " ++ local_strat_name) (tscript_string ps.tscript)
+-- ++ ps.unused ++ hints_string ps.hints 
+
+-- meta def output (s : string) : io unit := do 
+--   of ← io.mk_file_handle "src/evidence.lean" io.mode.write, 
+--   io.fs.write of s.to_char_buffer
+
+-- meta def driver (input : pexpr) : tactic unit := 
+-- let α := path fcs in 
+-- let ps : PROOF_STATE α := {} in 
+-- do 
+--   STRAT ← tactic.to_expr input,
+--   match STRAT with 
+--   | `(property.input.mk %%CLAIM %%PROPS) := 
+--   do 
+--   inpt ← tactic.eval_expr (property.input α) STRAT,
+--   input_fmt ← tactic_format_expr STRAT,
+--   let input_s := input_fmt.to_string, 
+--   let ps := { input := inpt, 
+--               input_string := input_s,
+--               strat_expr := STRAT , 
+--               PROPS := PROPS,
+--               -- TODO : Clean this
+--               init_goal := `(deductive (path fcs) (property.strategy %%STRAT)), 
+--               ..ps},
+--               -- And this
+--   let ps := get_originals ps,
+--   let goal_str := "deductive (path fcs) " ++ local_strat_name,
+--   set_goal ps.init_goal, 
+--   ps ← solve_inductive (ps),
+--   str ← get_unused ps,
+--     match ps.solved with 
+--     | tt := tactic.trace "True"
+--     | ff := tactic.trace "False"
+--     end,
+--     tactic.unsafe_run_io $ output $ evidence_file_template {unused := str ..ps}
+-- | _ := return ()
+-- end
+
+
+-- @[user_command]
+-- meta def main
+-- (meta_info : decl_meta_info)
+-- (_ : parse (lean.parser.tk "main")) : lean.parser unit :=
+-- do 
+--    F ← read "src/input/Inductive_Example.txt" types.texpr,
+--    lean.parser.of_tactic $ driver F
+-- . 
