src/property_catalogue/LTL/sat/absent.lean
@@ -1,4 +1,4 @@
-import LTS property_catalogue.LTL.patterns tactic common_meta
+import LTS property_catalogue.LTL.patterns tactic 
 
 open tactic
 
@@ -55,4 +55,93 @@ meta def solve (tok : expr) (str : string) : list expr → tactic unit
 
 
 end globally 
+
+
+namespace between
+
+theorem absent_between_response {M : LTS} {p : path M} { B I C : formula M} ( A : formula M) : 
+(sat (responds.globally  (C) (A) ) p) ∧ 
+(sat (absent.between (B) (C) (A)) p) ∧  
+(sat (absent.between (B) (A) (I)) p)→ (sat (absent.between (B) (C) (I)) p) := 
+begin rintros ⟨ H1, H2, H3⟩,
+intro i,
+replace H1 := H1 i,
+intro Hcond, cases Hcond with L R,
+replace H1 := H1 L,
+rw absent.between at H2,
+have : ((p.drop i) ⊨ (C &  ◆A)), by {rw sat, split,assumption,assumption},
+replace H2 := H2 (i) this,
+cases H1 with w Hw,
+cases R with k Hk,
+clear this,
+cases H2 with z Hz,
+cases Hz with z1 z2,
+have : k < z ∨ ¬ (k < z), from or_not,
+cases this, 
+use k,
+split, assumption,
+intros j Hj,
+have fact : j < z, by omega,
+replace z2 := z2 j fact, assumption,
+simp at this,
+have EM : z = k ∨ z < k, by omega,
+clear this,
+cases EM, use k,
+split, assumption, rw ← EM, assumption,
+replace H3 := H3 (i+z),
+rw ← path.drop_drop at H3,
+have help : (((p.drop i).drop z) ⊨ ◆(I)), by {use (k-z),
+rw path.drop_drop, rw path.drop_drop,have : i + (z + (k - z)) = i+k, by omega, rw this, rw ← path.drop_drop, assumption,},
+have : ( ((p.drop i).drop z) ⊨  (A &  ◆I)), by {rw sat, split, assumption, assumption,},
+clear help, replace H3 := H3 this,
+cases H3 with t Ht,
+clear this,
+cases Ht with Ht Ht',
+rw path.drop_drop at *,
+use (z+t),split,
+assumption,
+intros j Hj,
+have : j < z ∨ ¬ (j < z), from or_not,
+cases this, replace z2 := z2 j this,
+assumption,
+simp at this,
+have EM' : z = j ∨ z < j, by omega,
+cases EM', rw EM' at Hj,
+replace Ht' := Ht' 0 _,
+rw path.drop_drop at Ht',
+rw← EM',
+simp at Ht', rw path.drop_drop,assumption,
+omega,
+clear this,
+replace Ht' := Ht' (j-z),
+rw path.drop_drop at Ht',
+have : (i + z + (j - z)) = (i + j), by omega,
+rw this at Ht',
+rw path.drop_drop,
+ apply Ht', omega,
+end 
+
+
+meta def solve_by_absent_between_response (A : expr) : tactic unit := 
+do 
+  tactic.interactive.apply ``(absent_between_response %%A),
+  repeat1 (applyc `and.intro), `[repeat {assumption}]
+
+meta def solve  (str : string) : list expr → tactic unit 
+| [] :=  return ()
+| (h::t) := 
+   do typ ← infer_type h,
+   match typ with 
+   | `(sat (responds.globally %%C %%A) _):=
+     solve_by_absent_between_response A <|> solve t
+   | _ := do solve t 
+   end 
+
+
+
+end between 
+
+
 end absent 
+
+
